# Binomial Expansion
**Def**: if $n$ & $k$ are integers such that $k \le n$ then we define a **Binomial coefficient**
## $$\binom nk = \dfrac{n!}{k! \cdot (n-k)!}$$
and we read $\binom nk$ as "n choose k"
# Binomial Theorem
$$\binom n 0 = \dfrac{n!}{0! \cdot (n-0)!} = \dfrac{n!}{n!} = 1$$
$$\binom n 1  = \dfrac{n!}{1! \cdot (n-1)!} = \dfrac{n(n-1)!}{(n-1!)} = n$$
$$\binom n n  = \dfrac{n!}{n! \cdot (n-n!)} = 1$$
- The expression $(a+b)$ is called a binomial, and $(a+b)^b$ is called the $n^{th}$ power of a binomial
- we have: 
$$(a +b)^1 = a + b$$
$$($$